refactor(data/list/{alist,sigma},data/finmap): renaming
* knodup -> nodupkeys
* val -> entries
* nd -> nodupkeys

data/finmap.lean
@@ -13,29 +13,29 @@ open list
 namespace multiset
 variables {α : Type*} {β : α → Type*}
 
-/-- `knodup s` means that `s` has no duplicate keys. -/
-def knodup (s : multiset (sigma β)) : Prop :=
-quot.lift_on s list.knodup (λ s t p, propext $ perm_knodup p)
+/-- `nodupkeys s` means that `s` has no duplicate keys. -/
+def nodupkeys (s : multiset (sigma β)) : Prop :=
+quot.lift_on s list.nodupkeys (λ s t p, propext $ perm_nodupkeys p)
 
-@[simp] theorem coe_knodup {l : list (sigma β)} : @knodup α β l ↔ l.knodup := iff.rfl
+@[simp] theorem coe_nodupkeys {l : list (sigma β)} : @nodupkeys α β l ↔ l.nodupkeys := iff.rfl
 
 end multiset
 
 /-- `finmap α β` is the type of finite maps over a multiset. It is effectively
   a quotient of `alist α β` by permutation of the underlying list. -/
 structure finmap (α : Type u) (β : α → Type v) : Type (max u v) :=
-(val : multiset (sigma β))
-(nd : val.knodup)
+(entries : multiset (sigma β))
+(nodupkeys : entries.nodupkeys)
 
 /-- The quotient map from `alist` to `finmap`. -/
-def alist.to_finmap {α β} (s : alist α β) : finmap α β := ⟨s.val, s.nd⟩
+def alist.to_finmap {α β} (s : alist α β) : finmap α β := ⟨s.entries, s.nodupkeys⟩
 local notation `⟦`:max a `⟧`:0 := alist.to_finmap a
 
 theorem alist.to_finmap_eq {α β} {s₁ s₂ : alist α β} :
-  ⟦s₁⟧ = ⟦s₂⟧ ↔ s₁.val ~ s₂.val :=
+  ⟦s₁⟧ = ⟦s₂⟧ ↔ s₁.entries ~ s₂.entries :=
 by cases s₁; cases s₂; simp [alist.to_finmap]
 
-@[simp] theorem alist.to_finmap_val {α β} (s : alist α β) : ⟦s⟧.val = s.val := rfl
+@[simp] theorem alist.to_finmap_entries {α β} (s : alist α β) : ⟦s⟧.entries = s.entries := rfl
 
 namespace finmap
 variables {α : Type u} {β : α → Type v}
@@ -44,12 +44,12 @@ open alist
 /-- Lift a permutation-respecting function on `alist` to `finmap`. -/
 @[elab_as_eliminator] def lift_on
   {γ} (s : finmap α β) (f : alist α β → γ)
-  (H : ∀ a b : alist α β, a.val ~ b.val → f a = f b) : γ :=
+  (H : ∀ a b : alist α β, a.entries ~ b.entries → f a = f b) : γ :=
 begin
   refine (quotient.lift_on s.1 (λ l, (⟨_, λ nd, f ⟨l, nd⟩⟩ : roption γ))
-    (λ l₁ l₂ p, roption.ext' (perm_knodup p) _) : roption γ).get _,
+    (λ l₁ l₂ p, roption.ext' (perm_nodupkeys p) _) : roption γ).get _,
   { exact λ h₁ h₂, H _ _ (by exact p) },
-  { have := s.nd, rcases s.val with ⟨l⟩, exact id }
+  { have := s.nodupkeys, rcases s.entries with ⟨l⟩, exact id }
 end
 
 @[simp] theorem lift_on_to_finmap {γ} (s : alist α β) (f : alist α β → γ) (H) :
@@ -59,20 +59,20 @@ end
   {C : finmap α β → Prop} (s : finmap α β) (H : ∀ a, C ⟦a⟧) : C s :=
 by rcases s with ⟨⟨a⟩, h⟩; exact H ⟨a, h⟩
 
-@[extensionality] theorem ext : ∀ {s t : finmap α β}, s.val = t.val → s = t
+@[extensionality] theorem ext : ∀ {s t : finmap α β}, s.entries = t.entries → s = t
 | ⟨l₁, h₁⟩ ⟨l₂, h₂⟩ H := by congr'
 
 /-- The predicate `a ∈ s` means that `s` has a value associated to the key `a`. -/
-instance : has_mem α (finmap α β) := ⟨λ a s, ∃ b : β a, sigma.mk a b ∈ s.val⟩
+instance : has_mem α (finmap α β) := ⟨λ a s, ∃ b : β a, sigma.mk a b ∈ s.entries⟩
 
 theorem mem_def {a : α} {s : finmap α β} :
-  a ∈ s ↔ ∃ b : β a, sigma.mk a b ∈ s.val := iff.rfl
+  a ∈ s ↔ ∃ b : β a, sigma.mk a b ∈ s.entries := iff.rfl
 
 @[simp] theorem mem_to_finmap {a : α} {s : alist α β} :
   a ∈ ⟦s⟧ ↔ a ∈ s := iff.rfl
 
 /-- The list of keys of a finite map. -/
-def keys (s : finmap α β) : multiset α := s.val.map sigma.fst
+def keys (s : finmap α β) : multiset α := s.entries.map sigma.fst
 
 @[simp] theorem keys_to_finmap (s : alist α β) :
   keys ⟦s⟧ = s.keys := rfl
@@ -84,22 +84,22 @@ theorem keys_nodup (s : finmap α β) : s.keys.nodup :=
 induction_on s $ λ s, s.keys_nodup
 
 /-- The empty map. -/
-instance : has_emptyc (finmap α β) := ⟨⟨0, knodup_nil⟩⟩
+instance : has_emptyc (finmap α β) := ⟨⟨0, nodupkeys_nil⟩⟩
 
 @[simp] theorem empty_to_finmap (s : alist α β) :
   (⟦∅⟧ : finmap α β) = ∅ := rfl
 
-theorem not_mem_empty_val {s : sigma β} : s ∉ (∅ : finmap α β).val :=
+theorem not_mem_empty_entries {s : sigma β} : s ∉ (∅ : finmap α β).entries :=
 multiset.not_mem_zero _
 
 theorem not_mem_empty {a : α} : a ∉ (∅ : finmap α β) :=
-λ ⟨b, h⟩, not_mem_empty_val h
+λ ⟨b, h⟩, not_mem_empty_entries h
 
 @[simp] theorem keys_empty : (∅ : finmap α β).keys = 0 := rfl
 
 /-- The singleton map. -/
 def singleton (a : α) (b : β a) : finmap α β :=
-⟨⟨a, b⟩::0, knodup_singleton _⟩
+⟨⟨a, b⟩::0, nodupkeys_singleton _⟩
 
 @[simp] theorem keys_singleton (a : α) (b : β a) : (singleton a b).keys = [a] := rfl
 
@@ -133,10 +133,10 @@ lift_on s (λ t, ⟦insert a b t⟧) $
 induction_on s $ λ ⟨s, nd⟩ h, congr_arg to_finmap $
 insert_of_pos (mem_to_finmap.2 h)
 
-theorem insert_val_of_neg {a : α} {b : β a} {s : finmap α β} : a ∉ s →
-  (insert a b s).val = ⟨a, b⟩ :: s.val :=
+theorem insert_entries_of_neg {a : α} {b : β a} {s : finmap α β} : a ∉ s →
+  (insert a b s).entries = ⟨a, b⟩ :: s.entries :=
 induction_on s $ λ s h,
-by simp [insert_val_of_neg (mt mem_to_finmap.1 h)]
+by simp [insert_entries_of_neg (mt mem_to_finmap.1 h)]
 
 @[simp] theorem keys_insert (a : α) (b : β a) (s : finmap α β) :
   (insert a b s).keys = s.keys.ndinsert a :=
@@ -167,7 +167,7 @@ induction_on s $ λ s, by simp
 def foldl {δ : Type w} (f : δ → Π a, β a → δ)
   (H : ∀ d a₁ b₁ a₂ b₂, f (f d a₁ b₁) a₂ b₂ = f (f d a₂ b₂) a₁ b₁)
   (d : δ) (m : finmap α β) : δ :=
-m.val.foldl (λ d s, f d s.1 s.2) (λ d s t, H _ _ _ _ _) d
+m.entries.foldl (λ d s, f d s.1 s.2) (λ d s t, H _ _ _ _ _) d
 
 /-- Erase a key from the map. If the key is not present it does nothing. -/
 def erase (a : α) (s : finmap α β) : finmap α β :=
