data/list/alist.lean
@@ -14,47 +14,47 @@ open list
   It is a wrapper around certain `list` functions with the added constraint
   that the list have unique keys. -/
 structure alist (α : Type u) (β : α → Type v) : Type (max u v) :=
-(val : list (sigma β))
-(nd : val.knodup)
+(entries : list (sigma β))
+(nodupkeys : entries.nodupkeys)
 
 namespace alist
 variables {α : Type u} {β : α → Type v}
 
-@[extensionality] theorem ext : ∀ {s t : alist α β}, s.val = t.val → s = t
+@[extensionality] theorem ext : ∀ {s t : alist α β}, s.entries = t.entries → s = t
 | ⟨l₁, h₁⟩ ⟨l₂, h₂⟩ H := by congr'
 
 /-- The predicate `a ∈ s` means that `s` has a value associated to the key `a`. -/
-instance : has_mem α (alist α β) := ⟨λ a s, ∃ b : β a, sigma.mk a b ∈ s.val⟩
+instance : has_mem α (alist α β) := ⟨λ a s, ∃ b : β a, sigma.mk a b ∈ s.entries⟩
 
 theorem mem_def {a : α} {s : alist α β} :
-  a ∈ s ↔ ∃ b : β a, sigma.mk a b ∈ s.val := iff.rfl
+  a ∈ s ↔ ∃ b : β a, sigma.mk a b ∈ s.entries := iff.rfl
 
-theorem mem_of_perm {a : α} {s₁ s₂ : alist α β} (p : s₁.val ~ s₂.val) : a ∈ s₁ ↔ a ∈ s₂ :=
+theorem mem_of_perm {a : α} {s₁ s₂ : alist α β} (p : s₁.entries ~ s₂.entries) : a ∈ s₁ ↔ a ∈ s₂ :=
 exists_congr $ λ b, mem_of_perm p
 
 /-- The list of keys of an association list. -/
-def keys (s : alist α β) : list α := s.val.map sigma.fst
+def keys (s : alist α β) : list α := s.entries.map sigma.fst
 
 theorem mem_keys {a : α} {s : alist α β} : a ∈ s.keys ↔ a ∈ s :=
 by rw [keys, mem_map]; exact
 ⟨λ ⟨⟨_, b⟩, h, rfl⟩, ⟨b, h⟩, λ ⟨b, h⟩, ⟨_, h, rfl⟩⟩
 
-theorem keys_nodup (s : alist α β) : s.keys.nodup := s.nd
+theorem keys_nodup (s : alist α β) : s.keys.nodup := s.nodupkeys
 
 /-- The empty association list. -/
-instance : has_emptyc (alist α β) := ⟨⟨[], knodup_nil⟩⟩
+instance : has_emptyc (alist α β) := ⟨⟨[], nodupkeys_nil⟩⟩
 
-theorem not_mem_empty_val {s : sigma β} : s ∉ (∅ : alist α β).val :=
+theorem not_mem_empty_entries {s : sigma β} : s ∉ (∅ : alist α β).entries :=
 not_mem_nil _
 
 theorem not_mem_empty {a : α} : a ∉ (∅ : alist α β) :=
-λ ⟨b, h⟩, not_mem_empty_val h
+λ ⟨b, h⟩, not_mem_empty_entries h
 
 @[simp] theorem keys_empty : (∅ : alist α β).keys = [] := rfl
 
 /-- The singleton association list. -/
 def singleton (a : α) (b : β a) : alist α β :=
-⟨[⟨a, b⟩], knodup_singleton _⟩
+⟨[⟨a, b⟩], nodupkeys_singleton _⟩
 
 @[simp] theorem keys_singleton (a : α) (b : β a) : (singleton a b).keys = [a] := rfl
 
@@ -62,14 +62,14 @@ variables [decidable_eq α]
 
 /-- Look up the value associated to a key in an association list. -/
 def lookup (a : α) (s : alist α β) : option (β a) :=
-s.val.lookup a
+s.entries.lookup a
 
 theorem lookup_is_some {a : α} {s : alist α β} :
   (s.lookup a).is_some ↔ a ∈ s := lookup_is_some
 
-theorem perm_lookup {a : α} {s₁ s₂ : alist α β} (p : s₁.val ~ s₂.val) :
+theorem perm_lookup {a : α} {s₁ s₂ : alist α β} (p : s₁.entries ~ s₂.entries) :
   s₁.lookup a = s₂.lookup a :=
-perm_lookup _ s₁.nd s₂.nd p
+perm_lookup _ s₁.nodupkeys s₂.nodupkeys p
 
 instance (a : α) (s : alist α β) : decidable (a ∈ s) :=
 decidable_of_iff _ lookup_is_some
@@ -77,21 +77,21 @@ decidable_of_iff _ lookup_is_some
 /-- Insert a key-value pair into an association list.
   If the key is already present it does nothing. -/
 def insert (a : α) (b : β a) (s : alist α β) : alist α β :=
-if h : a ∈ s then s else ⟨⟨a, b⟩ :: s.val,
-  nodup_cons.2 ⟨mt mem_keys.1 h, s.nd⟩⟩
+if h : a ∈ s then s else ⟨⟨a, b⟩ :: s.entries,
+  nodup_cons.2 ⟨mt mem_keys.1 h, s.nodupkeys⟩⟩
 
 @[simp] theorem insert_of_pos {a : α} {b : β a} {s : alist α β} (h : a ∈ s) :
   insert a b s = s := dif_pos h
 
-theorem insert_val_of_neg {a : α} {b : β a} {s : alist α β} (h : a ∉ s) :
-  (insert a b s).val = ⟨a, b⟩ :: s.val := by simp [insert, h]
+theorem insert_entries_of_neg {a : α} {b : β a} {s : alist α β} (h : a ∉ s) :
+  (insert a b s).entries = ⟨a, b⟩ :: s.entries := by simp [insert, h]
 
 @[simp] theorem keys_insert (a : α) (b : β a) (s : alist α β) :
   (insert a b s).keys = _root_.insert a s.keys :=
 begin
   by_cases a ∈ s,
   { simp [h, mem_keys.2 h] },
-  { simp [keys, insert_val_of_neg h],
+  { simp [keys, insert_entries_of_neg h],
     exact (insert_of_not_mem (mt mem_keys.1 h)).symm }
 end
 
@@ -100,18 +100,18 @@ end
 by rw [← mem_keys, ← mem_keys]; simp
 
 theorem perm_insert {a : α} {b : β a} {s₁ s₂ : alist α β}
-  (p : s₁.val ~ s₂.val) : (insert a b s₁).val ~ (insert a b s₂).val :=
+  (p : s₁.entries ~ s₂.entries) : (insert a b s₁).entries ~ (insert a b s₂).entries :=
 begin
   by_cases a ∈ s₁,
   { simp [h, (mem_of_perm p).1 h, p] },
-  { simp [insert_val_of_neg h, insert_val_of_neg (mt (mem_of_perm p).2 h)],
+  { simp [insert_entries_of_neg h, insert_entries_of_neg (mt (mem_of_perm p).2 h)],
     exact p.skip _ }
 end
 
 /-- Replace a key with a given value in an association list.
   If the key is not present it does nothing. -/
 def replace (a : α) (b : β a) (s : alist α β) : alist α β :=
-⟨kreplace a b s.val, (kreplace_knodup a b).2 s.nd⟩
+⟨kreplace a b s.entries, (kreplace_nodupkeys a b).2 s.nodupkeys⟩
 
 @[simp] theorem keys_replace (a : α) (b : β a) (s : alist α β) :
   (replace a b s).keys = s.keys :=
@@ -122,16 +122,16 @@ kreplace_map_fst _ _ _
 by rw [← mem_keys, keys_replace, mem_keys]
 
 theorem perm_replace {a : α} {b : β a} {s₁ s₂ : alist α β} :
-  s₁.val ~ s₂.val → (replace a b s₁).val ~ (replace a b s₂).val :=
-perm_kreplace s₁.nd
+  s₁.entries ~ s₂.entries → (replace a b s₁).entries ~ (replace a b s₂).entries :=
+perm_kreplace s₁.nodupkeys
 
 /-- Fold a function over the key-value pairs in the map. -/
 def foldl {δ : Type w} (f : δ → Π a, β a → δ) (d : δ) (m : alist α β) : δ :=
-m.val.foldl (λ r a, f r a.1 a.2) d
+m.entries.foldl (λ r a, f r a.1 a.2) d
 
 /-- Erase a key from the map. If the key is not present it does nothing. -/
 def erase (a : α) (s : alist α β) : alist α β :=
-⟨kerase a s.val, kerase_knodup _ s.nd⟩
+⟨kerase a s.entries, kerase_nodupkeys _ s.nodupkeys⟩
 
 @[simp] theorem keys_erase (a : α) (s : alist α β) :
   (erase a s).keys = s.keys.erase a :=
@@ -141,14 +141,14 @@ by rw [erase_eq_erasep, keys, keys, erasep_map]; refl
 by rw [← mem_keys, keys_erase, mem_erase_iff_of_nodup s.keys_nodup, mem_keys]
 
 theorem perm_erase {a : α} {s₁ s₂ : alist α β} :
-  s₁.val ~ s₂.val → (erase a s₁).val ~ (erase a s₂).val :=
-perm_kerase s₁.nd
+  s₁.entries ~ s₂.entries → (erase a s₁).entries ~ (erase a s₂).entries :=
+perm_kerase s₁.nodupkeys
 
 /-- Erase a key from the map, and return the corresponding value, if found. -/
 def extract (a : α) (s : alist α β) : option (β a) × alist α β :=
-have (kextract a s.val).2.knodup,
-by rw [kextract_eq_lookup_kerase]; exact kerase_knodup _ s.nd,
-match kextract a s.val, this with
+have (kextract a s.entries).2.nodupkeys,
+by rw [kextract_eq_lookup_kerase]; exact kerase_nodupkeys _ s.nodupkeys,
+match kextract a s.entries, this with
 | (b, l), h := (b, ⟨l, h⟩)
 end
 
